aneris/examples/crdt/oplib/examples/prod_comb/prod_comb_proof.v
@@ -369,4 +369,5 @@ Section prod_proof.
       eauto with iFrame.
     Qed.
 
+
 End prod_proof.
