aneris/examples/crdt/statelib/examples/gcounter/gcounter_code_wrapper.v
@@ -1,0 +1,52 @@
+From aneris.aneris_lang Require Import ast aneris_lifting.
+From aneris.aneris_lang.lib Require Import list_code.
+From aneris.aneris_lang.lib.vector_clock Require Import vector_clock_code.
+From aneris.examples.crdt.statelib Require Import statelib_code.
+From aneris.examples.crdt.spec Require Import crdt_base.
+
+Section gcpt_code_wrapper.
+
+  Context `{!CRDT_Params}.
+
+  Definition gcpt_init_st : val :=
+    λ: <>, vect_make #(length CRDT_Addresses) #0.
+
+Definition list_map2 : val :=
+  rec: "list_map2" "f" "l" "l'" :=
+  match: "l" with
+    SOME "a" =>
+    match: "l'" with
+      SOME "b" =>
+      "f" (Fst "a") (Fst "b") :: "list_map2" "f" (Snd "a") (Snd "b")
+    | NONE => assert: #false
+    end
+  | NONE => NONE
+  end.
+
+Definition gcpt_mutator : val :=
+  λ: "repId" "st" "op",
+  match: list_nth "st" "repId" with
+    NONE => "st"
+  | SOME "p" => vect_update "st" "repId" ("op" + "p")
+  end.
+
+Definition max_fn : val := λ: "i" "j", (if: "i" < "j"
+                            then  "j"
+                            else  "i").
+
+Definition gcpt_merge : val := λ: "st" "st'", list_map2 max_fn "st" "st'".
+
+Definition gcpt_crdt : val :=
+    λ: <>, ((gcpt_init_st, gcpt_mutator), gcpt_merge).
+
+Definition gcpt_init : val :=
+  λ: "addrs" "rid",
+  let: "len" := list_length "addrs" in
+  let: "initRes" := statelib_init
+                      vect_serialize vect_deserialize
+                      "addrs" "rid" gcpt_crdt in
+  let: "get_state" := Fst "initRes" in
+  let: "update" := Snd "initRes" in
+  ("get_state", "update").
+
+End gcpt_code_wrapper.
