aneris/examples/crdt/statelib/examples/pncounter/pncounter_code_wrapper.v
@@ -1,0 +1,68 @@
+From aneris.aneris_lang Require Import ast aneris_lifting.
+From aneris.aneris_lang.lib Require Import list_code.
+From aneris.aneris_lang.lib.vector_clock Require Import vector_clock_code.
+From aneris.examples.crdt.statelib Require Import statelib_code.
+From aneris.examples.crdt.spec Require Import crdt_base.
+From aneris.examples.crdt.statelib.examples.gcounter
+     Require Import gcounter_code_wrapper.
+From aneris.examples.crdt.statelib.examples.prod_comb
+     Require Import prod_comb_code.
+
+Section pn_cpt_code_wrapper.
+
+  Context `{!CRDT_Params}.
+
+  (**  Step 1. Raw PN counter using product and gcpt crdts.  *)
+
+  Definition pn_cpt_init_st : val :=
+    λ: <>, prod_init_st gcpt_init_st gcpt_init_st #().
+
+  Definition pn_cpt_mutator : val :=
+    λ: "i" "gs" "op",
+   prod_mutator gcpt_mutator gcpt_mutator "i" "gs" "op".
+
+  Definition pn_cpt_merge : val :=
+  λ: "st1" "st2", prod_merge gcpt_merge gcpt_merge "st1" "st2".
+
+  Definition pn_cpt_crdt : val :=
+    λ: <>, prod_crdt gcpt_crdt gcpt_crdt #().
+
+  Definition pn_cpt_init : val :=
+    λ: "addrs" "rid",
+      prod_init
+        vect_serialize vect_deserialize
+        vect_serialize vect_deserialize
+        gcpt_crdt gcpt_crdt "addrs" "rid".
+
+  (**  Step 2. PN counter wrapper.  *)
+
+  Definition list_int_sum : val :=
+    λ: "l", list_fold (λ: "acc" "n", "acc" + "n") #0 "l".
+
+
+  Definition pncounter_update : val :=
+    λ: "upd" "n",
+      (if: #0 ≤ "n"
+       then  "upd" ("n", #0)
+       else  "upd" (#0, (- "n"))).
+
+  Definition pncounter_eval : val :=
+    λ: "get_state" <>,
+       let: "st" := "get_state" #() in
+       let: "pl" := Fst "st" in
+       let: "nl" := Snd "st" in
+       let: "p" := list_int_sum "pl" in
+       let: "n" := list_int_sum "nl" in
+       "p" - "n".
+
+
+  Definition pncounter_init : val :=
+    λ: "addrs" "rid",
+      let: "pn_cpt" := pn_cpt_init "addrs" "rid" in
+      let: "get_st" := Fst "pn_cpt" in
+      let: "upd_st" := Snd "pn_cpt" in
+      let: "get" := pncounter_eval "get_st" in
+      let: "upd" := pncounter_update "upd_st" in
+      ("get", "upd").
+
+End pn_cpt_code_wrapper.
