aneris/examples/crdt/statelib/examples/pncounter/pncounter_proof.v
@@ -1,0 +1,116 @@
+From Coq Require Import ssreflect Vector.
+From stdpp Require Import base gmap vector.
+From iris.proofmode Require Import tactics.
+From aneris.prelude Require Import gset_map.
+From aneris.prelude Require Import misc strings.
+From aneris.aneris_lang Require Import lang.
+From aneris.aneris_lang.lib Require Import network_util_proof.
+From aneris.aneris_lang.lib Require Import list_proof set_proof .
+From aneris.aneris_lang.lib.serialization Require Import serialization_proof.
+From aneris.aneris_lang Require Import aneris_lifting proofmode.
+From aneris.aneris_lang.lib.vector_clock Require Import vector_clock_code vector_clock_proof.
+From aneris.examples.crdt.spec Require Import crdt_base crdt_time crdt_events crdt_denot crdt_resources.
+From aneris.examples.crdt.statelib.user_model
+     Require Import semi_join_lattices model params.
+From aneris.examples.crdt.statelib.time Require Import time.
+From aneris.examples.crdt.statelib.STS Require Import lst.
+From aneris.examples.crdt.statelib.proof
+     Require Import events spec.
+From aneris.examples.crdt.statelib Require Import statelib_code.
+From aneris.examples.crdt.statelib.examples.gcounter
+     Require Import gcounter_code_wrapper gcounter_proof.
+From aneris.examples.crdt.statelib.examples.prod_comb
+     Require Import prod_comb_code prod_comb_proof.
+From aneris.examples.crdt.statelib.examples.pncounter
+     Require Import pncounter_code_wrapper.
+
+Section pn_cpt_proof.
+  Context `{!anerisG M Σ, !CRDT_Params, !StLib_Res (prodOp gctr_op gctr_op)}.
+
+  Notation pnOp := (prodOp gctr_op gctr_op).
+  Notation pnSt := (prodSt gctr_st gctr_st).
+  Notation pnParams := (prod_params gctr_op gctr_st gctr_op gctr_st).
+
+  Lemma pn_init_st_fn_spec :
+    ⊢ @init_st_fn_spec _ _ _ _ _ _ _ _ _ pnParams pn_cpt_init_st.
+  Proof.
+    iApply (prod_init_st_fn_spec $! gctr_init_st_fn_spec gctr_init_st_fn_spec).  Qed.
+
+  Lemma pn_cpt_mutator_spec :
+    ⊢ @mutator_spec _ _ _ _ _ _ _ _ _ pnParams pn_cpt_mutator.
+  Proof.
+    by iApply (prod_mutator_st_spec $! gctr_mutator_spec gctr_mutator_spec).
+  Qed.
+
+  Lemma pn_cpt_merge_spec :
+    ⊢ @merge_spec _ _ _ _ _ _ _ _ _ pnParams pn_cpt_merge.
+  Proof.
+    by iApply (prod_merge_st_spec $! gctr_merge_spec gctr_merge_spec).
+  Qed.
+
+  Lemma pn_crdt_fun_spec :
+    ⊢ @crdt_fun_spec _ _ _ _ _ _ _ _ _ pnParams pn_cpt_crdt.
+  Proof.
+    iApply (prod_crdt_fun_spec $! gctr_crdt_fun_spec gctr_crdt_fun_spec).
+  Qed.
+
+  Lemma pn_init_spec :
+    @init_spec
+      _ _ _ _ _ _ _ _ _ pnParams _
+      (statelib_init
+         (prod_ser
+            (gctr_params.(StLib_StSerialization).(s_serializer)).(s_ser)
+            (gctr_params.(StLib_StSerialization).(s_serializer)).(s_ser))
+         (prod_deser
+            (gctr_params.(StLib_StSerialization).(s_serializer)).(s_deser)
+            (gctr_params.(StLib_StSerialization).(s_serializer)).(s_deser))) -∗
+    @init_spec_for_specific_crdt
+      _ _ _ _ _ _ _ _ _ pnParams _
+       pn_cpt_init.
+  Proof.
+    iIntros "#Hinit".
+    by iApply (prod_init_spec $! gctr_crdt_fun_spec gctr_crdt_fun_spec with "[$Hinit]").
+  Qed.
+
+End pn_cpt_proof.
+
+Section pncounter_proof.
+
+  Context `{!anerisG M Σ, !CRDT_Params, !StLib_Res (prodOp gctr_op gctr_op)}.
+
+  Notation pnOp := (prodOp gctr_op gctr_op).
+  Notation pnSt := (prodSt gctr_st gctr_st).
+  Notation pnParams := (prod_params gctr_op gctr_st gctr_op gctr_st).
+
+  (* TODO: Prove: *)
+  (* Definition list_int_sum : val := *)
+    (* λ: "l", list_fold (λ: "acc" "n", "acc" + "n") #0 "l". *)
+
+  (* TODO: Prove: *)
+  (* Definition pncounter_update : val := *)
+  (*   λ: "upd" "n", *)
+  (*     (if: #0 ≤ "n" *)
+  (*      then  "upd" ("n", #0) *)
+  (*      else  "upd" (#0, (- "n"))). *)
+
+  (* TODO: Prove: *)
+  (* Definition pncounter_eval : val := *)
+  (*   λ: "get_state" <>, *)
+  (*      let: "st" := "get_state" #() in *)
+  (*      let: "pl" := Fst "st" in *)
+  (*      let: "nl" := Snd "st" in *)
+  (*      let: "p" := list_int_sum "pl" in *)
+  (*      let: "n" := list_int_sum "nl" in *)
+  (*      "p" - "n". *)
+
+  (* TODO: Prove: *)
+  (* Definition pncounter_init : val := *)
+  (*   λ: "addrs" "rid", *)
+  (*     let: "pn_cpt" := pn_cpt_init "addrs" "rid" in *)
+  (*     let: "get_st" := Fst "pn_cpt" in *)
+  (*     let: "upd_st" := Snd "pn_cpt" in *)
+  (*     let: "get" := pncounter_eval "get_st" in *)
+  (*     let: "upd" := pncounter_update "upd_st" in *)
+  (*     ("get", "upd"). *)
+
+End pncounter_proof.
